some proof for set_hash_alg with a couple of assumes

src/tls/HandshakeTranscript.fst
@@ -35,11 +35,12 @@ let region_of s = s.rgn
 unfold
 let footprint_locs (s:state) (h:HS.mem) =
   let open B in
-  [loc_buffer s.hash_state;
-   loc_buffer s.tx;
+  [
    (match deref h s.hash_state with
     | None -> loc_none
-    | Some (| _, hash_st |) -> IncHash.footprint hash_st h)]
+    | Some (| _, hash_st |) -> IncHash.footprint hash_st h);
+   loc_buffer s.hash_state;
+   loc_buffer s.tx;]
 
 unfold
 let footprint' (s:state) (h:HS.mem) =
@@ -96,7 +97,19 @@ let create r =
   let tx = B.malloc r (G.hide []) 1ul in
   { rgn = r; hash_state = hash_state; tx = tx }
 
-let set_hash_alg (s:state) = admit()
+let set_hash_alg a s =
+  let h0 = ST.get () in
+
+  let hash_st = IncHash.create_in a s.rgn in
+  B.upd s.hash_state 0ul (Some (| a, hash_st |));
+
+  let h2 = ST.get () in
+
+  assume (invariant s h2);
+  assume (B.(fresh_loc (IncHash.footprint hash_st h2) h0 h2))  //AR: the postcondition in IncHash is in terms of Hash.fresh_loc, that needs fixing
+
 let extend_hash s b p0 p1 msg = admit()
 let buf_is_hash_of_b (a:Hash.alg) (buf:Hacl.Hash.Definitions.hash_t a) (b:hbytes) : prop = admit()
 let extract_hash (#a:Hash.alg) (s:state) (tag:Hacl.Hash.Definitions.hash_t a) = admit()
+
+
